polygen/InstanceListSema.v
@@ -1,0 +1,178 @@
+(** instance list semantics *)
+
+Require Import Bool.
+Require Import Base.
+Require Import List.
+Require Import SetoidList.
+Require Import MSets.
+Require Import Coq.MSets.MSetProperties.
+Require Import Setoid Morphisms.
+Require Import Linalg.
+Require Import Base.
+Require Import LinalgExt.
+Require Import Classical.
+Require Import ZArith.
+Require Import PolyBase.
+Require Import Misc.
+Require Import Sorting.Sorted.
+Require Import Permutation.
+Require Import Coqlib.
+Require Import LibTactics.
+Require Import sflib.
+Import ListNotations.
+
+Require Import StateTy.
+Require Import InstrTy.
+
+Require Import AST.
+Require Import OpenScop.
+Require Import Result.
+
+Import ListNotations.
+
+Module ILSema (Instr: INSTR).
+
+Module State := Instr.State.
+
+Record InstrPoint := {
+  ip_nth: nat;  (** belongs to nth polyhedral instruction *)
+  ip_index: DomIndex;  (** index of the domain, i.e., iterator's value *)
+  ip_transformation: Transformation; (** transformation function *)
+  ip_time_stamp: TimeStamp;  (** schedule *)
+  ip_instruction: Instr.t;  (** basic instruction *)
+  ip_depth: nat;  (** surrounded iterator depth *)
+}.
+
+Definition eq_except_sched (ip1 ip2: InstrPoint): Prop := 
+  ip1.(ip_nth) = ip2.(ip_nth) /\ 
+  ip1.(ip_index) = ip2.(ip_index) /\ 
+  ip1.(ip_transformation) = ip2.(ip_transformation) /\
+  ip1.(ip_instruction) = ip2.(ip_instruction) /\ 
+  ip1.(ip_depth) = ip2.(ip_depth).
+
+Inductive instr_point_sema (ip: InstrPoint) 
+  (st1 st2: State.t): Prop :=
+  | ip_sema_intro: forall wcs rcs,
+    Instr.instr_semantics ip.(ip_instruction) 
+      (affine_product ip.(ip_transformation) ip.(ip_index)) wcs rcs st1 st2 -> 
+    instr_point_sema ip st1 st2.
+
+Definition instr_point_sched_le (ip1 ip2: InstrPoint): Prop := 
+  lex_compare ip1.(ip_time_stamp) ip2.(ip_time_stamp) = Lt \/ 
+  lex_compare ip1.(ip_time_stamp) ip2.(ip_time_stamp) = Eq. 
+
+Lemma instr_point_sched_le_trans:
+  forall ip1 ip2 ip3,
+    instr_point_sched_le ip1 ip2 ->
+    instr_point_sched_le ip2 ip3 ->
+    instr_point_sched_le ip1 ip3.
+Proof.
+  intros. unfolds instr_point_sched_le.
+  destruct H; destruct H0. 
+  - left. eapply lex_compare_trans; eauto.
+  - left.
+    rewrite <- is_eq_iff_cmp_eq in H0.
+    eapply lex_compare_right_eq with (t1:=ip_time_stamp ip1) in H0; eauto.
+    rewrite <- H0; trivial. 
+  - left.
+    rewrite <- is_eq_iff_cmp_eq in H.
+    eapply lex_compare_left_eq with (t3:=ip_time_stamp ip3) in H; eauto.
+    rewrite H; trivial.
+  - right. eapply lex_compare_trans; eauto.
+Qed. 
+
+
+Definition instr_point_sched_ltb (ip1 ip2: InstrPoint): bool := 
+  comparison_eqb (lex_compare ip1.(ip_time_stamp) ip2.(ip_time_stamp)) Lt.
+
+Definition instr_point_sched_eqb (ip1 ip2: InstrPoint): bool := 
+  comparison_eqb (lex_compare ip1.(ip_time_stamp) ip2.(ip_time_stamp)) Eq.
+
+
+Definition Permutable (ip1 ip2: InstrPoint) := 
+    forall st1, 
+        Instr.NonAlias st1 ->
+        (forall st2' st3,
+        instr_point_sema ip1 st1 st2' ->
+        instr_point_sema ip2 st2' st3 ->
+        exists st2'' st3',
+        instr_point_sema ip2 st1 st2'' /\
+        instr_point_sema ip1 st2'' st3' /\
+        Instr.State.eq st3 st3'
+        ) /\
+        (forall st2' st3,
+        instr_point_sema ip2 st1 st2' ->
+        instr_point_sema ip1 st2' st3 ->
+        exists st2'' st3',
+        instr_point_sema ip1 st1 st2'' /\
+        instr_point_sema ip2 st2'' st3' /\
+        Instr.State.eq st3 st3'
+        ).
+    
+Lemma Permutable_symm: 
+forall ip1 ip2, 
+    Permutable ip1 ip2 -> 
+    Permutable ip2 ip1.
+Proof.
+intros.
+unfolds Permutable.
+intros.
+split. 
+eapply H; eauto.
+eapply H; eauto.
+Qed.
+    
+Inductive instr_point_list_semantics: list InstrPoint ->
+State.t -> State.t -> Prop:=
+| IPLS_nil: forall st st', 
+Instr.State.eq st st' ->
+instr_point_list_semantics [] st st'
+| IPLS_cons: forall st1 st2 st3 ip il,
+instr_point_sema ip st1 st2 ->
+instr_point_list_semantics il st2 st3 ->
+instr_point_list_semantics (ip::il) st1 st3.
+
+Lemma instr_point_list_sema_stable_under_state_eq:
+  forall l st1 st2 st1' st2',
+    instr_point_list_semantics l st1 st2 ->
+    Instr.State.eq st1 st1' ->
+    Instr.State.eq st2 st2' ->
+    instr_point_list_semantics l st1' st2'.
+Proof.
+  induction l.
+  - 
+  intros. 
+  inv H. 
+  simpls. econs; eauto. 
+  eapply Instr.State.eq_sym in H0.
+  eapply Instr.State.eq_trans; eauto.
+  eapply Instr.State.eq_trans; eauto.
+  -
+  intros. inv H.
+  inv H4. 
+  eapply Instr.instr_semantics_stable_under_state_eq 
+    with (st1':=st1') (st2:=st3) (st2':=st3) in H; eauto.
+  2: {eapply Instr.State.eq_refl. }
+  econs; eauto. instantiate (1:=st3). econs; eauto.
+  eapply IHl; eauto. eapply Instr.State.eq_refl.  
+Qed.
+
+Definition veq_instance (ip1 ip2: InstrPoint): Prop :=
+  ip1.(ip_nth) = ip2.(ip_nth) 
+  /\ veq ip1.(ip_index) ip2.(ip_index) 
+  /\ ip1.(ip_transformation) = ip2.(ip_transformation)
+  /\ ip1.(ip_time_stamp) = ip2.(ip_time_stamp)
+  /\ ip1.(ip_instruction) = ip2.(ip_instruction)
+  /\ ip1.(ip_depth) = ip2.(ip_depth)
+.
+
+Lemma veq_instance_refl:
+  forall ip,
+    veq_instance ip ip.
+Proof.
+  intros. destruct ip. unfold veq_instance; splits; simpls; trivial.
+  eapply veq_refl.
+Qed.
+
+
+End ILSema.
